IMP/IMP_Base.thy
@@ -1,6 +1,6 @@
 \<^marker>\<open>creator Fabian Huch\<close>
 theory IMP_Base
-  imports Main
+  imports Eq_On
 begin
 
 type_synonym vname = string
@@ -27,6 +27,12 @@ text \<open>Variables, syntactic substitution, and maximum constant\<close>
 
 class vars =
   fixes vars :: "'a \<Rightarrow> vname list"
+begin
+
+lemma vars_finite[intro,simp]: "finite (set (vars x))"
+by simp
+
+end
 
 class subst = vars +
   fixes subst :: "(vname \<Rightarrow> vname) \<Rightarrow> 'a \<Rightarrow> 'a"
@@ -34,5 +40,38 @@ class subst = vars +
 
 class max_const =
   fixes max_const :: "'a \<Rightarrow> nat"
+
+definition max_state :: "vname list \<Rightarrow> state \<Rightarrow> nat" where
+  "max_state vrs s \<equiv> foldr (\<lambda>x. max (s x)) vrs 0"
+
+lemma max_state_empty[simp]: "max_state [] s = 0"
+  unfolding max_state_def by simp
+
+lemma max_state_cons[simp]: "max_state (x#xs) s = max (s x) (max_state xs s)"
+  unfolding max_state_def by simp
+
+lemma max_state_concat[simp]: "max_state (as @ bs) s = max (max_state as s) (max_state bs s)"
+  by (induction as) (auto simp: max_state_def)
+
+lemma max_state_upd[simp]: "max_state xs (s(x := y)) \<le> max y (max_state xs s)"
+  by (induction xs) auto
+
+lemma max_state_nonintf[simp]: "x \<notin> set xs \<Longrightarrow> max_state xs (s(x := y)) = max_state xs s"
+  by (induction xs) auto
+
+lemma max_state_part[simp,intro]: "s = s' on set vs \<Longrightarrow> max_state vs s = max_state vs s'"
+  unfolding max_state_def by (induction vs) (auto simp: eq_on_def)
+
+
+definition max_exp :: "'a::{max_const,vars} \<Rightarrow> state \<Rightarrow> nat" where
+  "max_exp e s = max (max_const e) (max_state (vars e) s)"
+
+
+fun num_bits :: "nat \<Rightarrow> nat" where
+"num_bits 0 = 0" |
+"num_bits n = Suc (num_bits (n div 2))"
+
+lemma num_bits_double[simp]: "num_bits (n + n) \<le> Suc (num_bits n)"
+  by (induction n rule: num_bits.induct) auto
 
 end
